\begin{center}

Lecture 4

\end{center}

If $X_i$ are extensive variables (other than $U$ and $S$). Define $Z_i = \frac{\partial S}{\partial X_i}$ and $Y_i = \frac{\partial U}{\partial X_i}$.

Maxwell relations are simply: $$\frac{\partial Y_i}{\partial X_j} = \frac{\partial Y_j}{\partial X_i}$$ and $$\frac{\partial Y_i}{\partial Y_j} = - \frac{\partial X_j}{\partial X_i}$$

\subsection{Specific heat, susceptibilities etc}

Specific heat: Measures change in entropy (equivalently by Claussius' relation the change in heat) with respect to temperature $C = T \frac{\partial S}{\partial T}$. Specific heat at a fixed volume: $T \left(\frac{\partial S}{\partial T}\right)_V$ and at a fixed pressure: $T \left(\frac{\partial S}{\partial T}\right)_P$.

We can also define specific heat directly from thermodynamic potentials: $$C_v = \left(\frac{\partial U}{\partial T}\right)_V$$ this follows from the first law $dU = TdS - PdV$ $$\implies \, \, \, \, \left(\frac{\partial U}{\partial T}\right)_V = T \left(\frac{\partial S}{\partial T}\right)_V$$

Susceptibility: If $(X,Y)$ are a pair of conjugate extensive-intensive variables: $$\xi = \frac{\partial X}{\partial Y}$$

Compressibility: $(P,V)$ with $$\kappa = - \frac{1}{V} \frac{\partial V}{\partial P}$$ usually we distinguish $$\kappa_T = - \frac{1}{V} \left(\frac{\partial V}{\partial P}\right)_T$$ as isothermal compressibility and $$\kappa_S = - \frac{1}{V} \left(\frac{\partial V}{\partial P}\right)_S$$ is adiabatic compressibility.

We call a constant $T$ isothermal and $S$ constant adiabatic (isentropic). $dS = 0 \implies \delta Q = 0$ by Claussius relation. 

\subsubsection*{Example: Q3 from problem sheet}

$S=c(UNV)^{1/3}$ derive the relations between $T, P, \mu$ and the extensive parameters.

\vspace{\baselineskip}

The first law states: $dU = TdS - PdV + \mu dN$

From these: $$T = \left(\frac{\partial U}{\partial S}\right)_{V,N}$$
$$P = - \left(\frac{\partial U}{\partial V}\right)_{S,N}$$
$$\mu = \left(\frac{\partial U}{\partial N}\right)_{S,V}$$

Now we can work out: $$U = \frac{S^3}{c^3 VN} = \alpha \frac{S^3}{VN}$$
$$T = 3 \alpha \frac{S^2}{VN} \implies T^3 = (3\alpha)^3 \frac{S^6}{(VN)^3}$$
$$P = \alpha \frac{S^3}{V^2 N} \implies P^2 = \frac{\alpha^2 S^6}{(V^2 N)^2}$$
$$\mu = - \alpha \frac{S^3}{VN^2}$$

Now using these we can get $$P = \sqrt{\frac{T^3N}{9 \alpha V}}$$ and $$\mu = - \sqrt{\frac{T^3 V}{3^3 \alpha N}}$$ and $$P = -\mu \frac{N}{V}$$

\subsubsection*{Example}

Show $$C_P - C_V = \frac{T V \alpha^2}{\kappa_T}$$

With $\kappa_T = - \frac{1}{V} \left(\frac{\partial V}{\partial P}\right)_T$ and $\alpha = \frac{1}{V} \frac{\partial V}{\partial T}$ and $C_P = T \left(\frac{\partial S}{\partial T}\right)_P$ and $C_V = T \left(\frac{\partial S}{\partial T}\right)_V$.

Start from the first law (with $\mu = 0$). $dU = TdS - PdV \implies TdS = dU + PdV$

Using $C_p = \left(\frac{\partial U}{\partial T}\right)_P$ and $C_V = \left(\frac{\partial U}{\partial T}\right)_V$ we see that $$TdS = C_V dT + T \left(\frac{\partial P}{\partial T}\right)_V dV$$ and $$TdS = C_P dT - T \left(\frac{\partial V}{\partial T}\right)_V dP$$.

Now using the chain rule for partials: $$\left(\frac{\partial P}{\partial T}\right)_V = - \frac{1}{\left(\frac{\partial T}{\partial V}\right)_P \left(\frac{\partial V}{\partial P}\right)_T} = \frac{\alpha}{\kappa_T}$$

So $TdS = C_V dT + \frac{\alpha T}{\kappa_T} dV$ and thus $TdS = C_P dT - \alpha TV dP$ now eliminate $dS$: $$(C_P - C_V) dT = \frac{\alpha T}{\kappa_T} dV + \alpha TV dP$$

If we treat $V$ and $P$ as independent variables: $$dT = \left(\frac{\partial T}{\partial V}\right)_P dV + \left(\frac{\partial T}{\partial P}\right)_V dP$$

So: $$\left[ (C_P - C_V) \left(\frac{\partial T}{\partial V}\right)_P - T \left(\frac{\partial P}{\partial T}\right)_V \right] + \left[(C_P - C_V) \left(\frac{\partial T}{\partial P}\right)_V - \left(\frac{\partial V}{\partial T}\right)_P \right] = 0$$

Now use the independence of $P,V$. This implies the coefficients of the exact differentials $dP, dV$ have to vanish: 
$$C_P - C_V = \frac{T \left(\frac{\partial P}{\partial T}\right)_V}{\left(\frac{\partial T}{\partial V}\right)_P} = \frac{T \alpha^2 V}{\kappa_T}$$